rustexamples/intrusive_linked_list/doubly_linked_list/main.rs
@@ -1,4 +1,3 @@
-
 struct Node{
     val: i32;
     link: Link;
@@ -15,6 +14,7 @@ fn link_offset() -> u64{
 }
 
 fn create(v: i32) -> Box<Node> {
+    // We can call an assembly program to encrypt the value and then store it to the list. The pop functions can decrypt the value.
     let head : Box<Node> = Box(Node{val: v, link: empty_link()});
     return create_link(head);
 }
@@ -23,4 +23,9 @@ fn push(l: Box<Node>, v: i32) -> Box<Node> {
     let head: Box<Node> = Box(Node {val: v, link: empty_link()});
     l = push_front(l, head);
     return l;
+}
+
+struct Option{
+    None,
+    Some(i32, Box<Node>)
 }
